examples/dsls/mini_steel/Pulse.Soundness.Return.fsti
@@ -1,14 +1,70 @@
 module Pulse.Soundness.Return
-module RT = Refl.Typing
-module R = FStar.Reflection
-module L = FStar.List.Tot
-module T = FStar.Tactics
-open FStar.List.Tot
-open Pulse.Syntax
+
+open FStar.Reflection
+open Refl.Typing
 open Pulse.Elaborate.Pure
+open Pulse.Elaborate.Core
 open Pulse.Typing
-open Pulse.Elaborate
 open Pulse.Soundness.Common
+
+module EPure = Pulse.Elaborate.Pure
+module RT = Refl.Typing
+
+
+let return_post_with_eq (u:universe) (a:term) (x:term) (p:term) : term =
+  let eq2_tm =
+    let t = pack_ln (Tv_UInst (pack_fv (mk_steel_wrapper_lid "eq2_prop")) [u]) in
+    let t = pack_ln (Tv_App t (a, Q_Implicit)) in
+    let t = pack_ln (Tv_App t (bound_var 0, Q_Explicit)) in
+    pack_ln (Tv_App t (x, Q_Explicit)) in
+
+  let p_app_0 = pack_ln (Tv_App p (bound_var 0, Q_Explicit)) in
+  
+  let star_tm =
+    let t = pack_ln (Tv_FVar (pack_fv star_lid)) in
+    let t = pack_ln (Tv_App t (p_app_0, Q_Explicit)) in
+    pack_ln (Tv_App t (eq2_tm, Q_Explicit)) in
+
+  mk_abs a Q_Explicit star_tm
+  
+val return_stt_typing
+  (#f:stt_env)
+  (#g:env)
+  (#u:universe)
+  (#a:term)
+  (#x:term)
+  (#p:term)
+  (a_typing:RT.typing (extend_env_l f g) a (pack_ln (Tv_Type u)))
+  (x_typing:RT.typing (extend_env_l f g) x a)
+  (p_typing:RT.typing (extend_env_l f g) p (mk_arrow (a, Q_Explicit) vprop_tm))
+
+  : GTot (RT.typing (extend_env_l f g)
+                    (mk_stt_return u a x p)
+                    (mk_stt_comp u a
+                       (pack_ln (Tv_App p (x, Q_Explicit)))
+                       (return_post_with_eq u a x p)))
+
+val return_stt_noeq_typing
+  (#f:stt_env)
+  (#g:env)
+  (#u:universe)
+  (#a:term)
+  (#x:term)
+  (#p:term)
+  (a_typing:RT.typing (extend_env_l f g) a (pack_ln (Tv_Type u)))
+  (x_typing:RT.typing (extend_env_l f g) x a)
+  (p_typing:RT.typing (extend_env_l f g) p (mk_arrow (a, Q_Explicit) vprop_tm))
+
+  : GTot (RT.typing (extend_env_l f g)
+                    (mk_stt_return u a x p)
+                    (mk_stt_comp u a (pack_ln (Tv_App p (x, Q_Explicit))) p))
+
+                      
+  // : GTot (RT.typing (extend_env_l f g)
+  //                   (mk_stt_admit u a p q)
+  //                   (mk_stt_comp u a p q))
+
+
 
 // val elab_return_typing (#f:stt_env)
 //                        (#g:env)
