examples/dsls/mini_steel/Pulse.Soundness.fst
@@ -344,6 +344,7 @@ let if_soundness
     tot_typing_soundness b_typing in
   let g_then = (hyp, Inl (mk_eq2 U_zero tm_bool b tm_true))::g in
   let re1_typing
+
     : RT.typing (RT.extend_env (extend_env_l f g)
                                hyp
                                (RT.eq2 (R.pack_universe R.Uv_Zero)
@@ -454,6 +455,19 @@ let admit_soundess
   | STT_Ghost ->
     Admit.stt_ghost_admit_soundness rt_typing rpre_typing rpost_typing
 
+let return_soundess
+  (#f:stt_env)
+  (#g:env)
+  (#t:st_term)
+  (#c:comp)
+  (d:st_typing f g t c{T_Return? d})
+  : GTot (RT.typing (extend_env_l f g)
+                    (elab_st_typing d)
+                    (elab_comp c)) =
+
+  let T_Return _ ctag use_eq u t e post x t_typing e_typing post_typing = d in
+  admit ()
+
 #push-options "--query_stats --fuel 2 --ifuel 2"
 let rec soundness (f:stt_env)
                   (g:env)
@@ -502,7 +516,8 @@ let rec soundness (f:stt_env)
     | T_Equiv _ _ _ _ _ _ ->
       stequiv_soundness _ _ _ _ d soundness
 
-    | T_Return _ c use_eq u t e post x t_typing e_typing post_typing -> admit ()
+    | T_Return _ _ _ _ _ _ _ _ _ _ _ ->
+      return_soundess d
 
     | T_If _ _ _ _ _ _ _ _ _ _ _->
       let ct_soundness f g c uc (d':_ {d' << d}) =
